UTLC.v
@@ -1,0 +1,709 @@
+From mathcomp Require Import all_ssreflect.
+
+Definition var := nat.
+
+Inductive lterm : Set :=
+| Var (x : var)
+| App (M : lterm) (N : lterm)
+| Abs (x : var) (M : lterm).
+
+Fixpoint eq_lterm (M N : lterm) : bool :=
+  match M, N with
+  | Var x, Var y => x == y
+  | App P Q, App P' Q' => (eq_lterm P P') && (eq_lterm Q Q')
+  | Abs x P, Abs y P' => (x == y) && (eq_lterm P P')
+  | _, _ => false
+  end.
+
+Lemma eq_ltermP : Equality.axiom eq_lterm.
+Proof.
+  rewrite /Equality.axiom.
+  elim=> [x|M IHM N IHN|x M IHM] [y|M' N'|y M'] /=.
+  - case: (x==y) /eqP.
+    + move=> Heq. constructor. by apply: f_equal.
+    + move=> Hneq. constructor. move=> Heq. by injection Heq.
+  - constructor. by [].
+  - constructor. by [].
+  - constructor. by [].
+  - have: reflect (M = M') (eq_lterm M M') by [].
+    have: reflect (N = N') (eq_lterm N N') by [].
+    elim=> [eqNT | eqNF] [eqMT | eqMF] /=.
+    + constructor. by apply: f_equal2.
+    + constructor. move=> Heq. by injection Heq.
+    + constructor. move=> Heq. by injection Heq.
+    + constructor. move=> Heq. by injection Heq.
+  - constructor. by [].
+  - constructor. by [].
+  - constructor. by [].
+  - have: reflect (M = M') (eq_lterm M M') by [].
+    elim=> [eqMT | eqMF];
+    case: (x == y) /eqP => Heqxy /=.
+    + constructor. by apply: f_equal2.
+    + constructor. move=> Heq. by injection Heq.
+    + constructor. move=> Heq. by injection Heq.
+    + constructor. move=> Heq. by injection Heq.
+Qed.
+
+Definition lterm_eqMixin := Equality.Mixin eq_ltermP.
+Canonical lterm_eqType := @Equality.Pack lterm lterm_eqMixin.
+                                
+Definition varset := seq var. 
+Definition singleton (x : var) := [:: x].
+Definition remove (x : var) (S : varset) : varset :=
+  filter (fun y => x != y) S.
+
+Lemma in_remove : forall x S, x \notin (remove x S).
+Proof.
+  move=> x S.
+  rewrite /remove. apply/negP. 
+  rewrite mem_filter.
+  move/andP => [Heq _].
+  by move/eqP: Heq => Heq.
+Qed.
+
+Fixpoint freevars (M : lterm) : varset :=
+  match M with
+  | Var x => [:: x]
+  | App M N => (freevars M) ++ (freevars N)
+  | Abs x M => (remove x (freevars M))
+  end.
+
+Fixpoint subst (x : var) (N M : lterm) :=
+  match M with
+  | Var y => if x == y
+             then N
+             else Var y
+  | App P Q => App (subst x N P) (subst x N Q)
+  | Abs y P => if x == y
+               then Abs y P
+               else Abs y (subst x N P)
+  end.
+
+Lemma subst_notin_fv (x : var) N M : 
+  x \notin freevars M -> M = subst x N M.
+Proof.
+  elim: M => [y|P IHP Q IHQ|y P IHP].
+  - rewrite /in_mem /mem /= Bool.orb_false_r.
+    move/negbTE=> H. by rewrite H.
+  - rewrite /= mem_cat negb_or.
+    move/andP=> [HnP HnQ].
+      by rewrite {1}(IHP HnP) {1}(IHQ HnQ).
+  - rewrite /=. case E: (x == y).
+    + by [].
+    + rewrite /remove mem_filter negb_and -implybE.
+      move/implyP=> H.
+      move/negbT: E. rewrite eq_sym. move=> E.
+        by rewrite {1}(IHP (H E)).
+Qed.
+
+Section beta.
+  Inductive beta1 : lterm -> lterm -> Prop :=
+  | beta1_redex
+    : forall x M N, beta1 (App (Abs x M) N) (subst x N M)
+  | beta1_appl
+    : forall P P' Q, beta1 P P' -> beta1 (App P Q) (App P' Q)
+  | beta1_appr
+    : forall P Q Q', beta1 Q Q' -> beta1 (App P Q) (App P Q')
+  | beta1_abs
+    : forall x P P', beta1 P P' -> beta1 (Abs x P) (Abs x P').
+
+  Inductive beta : lterm -> lterm -> Prop :=
+  | beta_refl
+    : forall M, beta M M
+  | beta_step
+    : forall P Q R, beta P Q -> beta1 Q R -> beta P R.
+
+  Notation "M -->b N" := (beta1 M N) (at level 70, no associativity).
+  Notation "M -->b* N" := (beta M N) (at level 70, no associativity).
+
+  Lemma beta1_beta : forall M N, M -->b N -> M -->b* N.
+  Proof.
+    move=> M N H.
+    apply: (beta_step M M N).
+    - by constructor.
+    - by [].
+  Qed.
+
+  Lemma beta_left : forall P Q R, P -->b Q -> Q -->b* R -> P -->b* R.
+  Proof.
+    move=> P Q R H1 H2. move: H2 H1. elim.
+    - by apply: beta1_beta.
+    - move=> P' Q' R' H1 H2 H3 H4.
+      apply: (beta_step _ Q').
+      + by apply: H2.
+      + by [].
+  Qed. 
+
+  Lemma beta_transitive : forall P Q R,
+      P -->b* Q -> Q -->b* R ->
+      P -->b* R.
+  Proof.
+    move=> P Q R. elim.
+    - by [].
+    - move=> P' Q' R' H1 H2 H3 H4.
+      apply: H2. by apply: (beta_left _ R').
+  Qed.
+
+  Lemma beta_stable_appl :
+    forall M M' N, M -->b* M' -> App M N -->b* App M' N.
+  Proof.
+    move=> M M' N. elim=> [P|P Q R IH].
+    - by constructor.
+    - move=> H1 H2.
+      have: App Q N -->b App R N by constructor.
+        by apply: (beta_step _ (App Q N) _).
+  Qed.
+
+  Lemma beta_stable_appr :
+    forall M N N', N -->b* N' -> App M N -->b* App M N'.
+  Proof.
+    move=> M N N'. elim=> [P|P Q R IH].
+    - by constructor.
+    - move=> H1 H2.
+      have: App M Q -->b App M R by constructor.
+        by apply: (beta_step _ (App M Q) _).
+  Qed.
+
+  Lemma beta_stable_abs :
+    forall x M M', M -->b* M' -> Abs x M -->b* Abs x M'.
+  Proof.
+    move=> x M M'. elim=> [P| P Q R IH].
+    - by constructor.
+    - move=> H1 H2.
+      have: Abs x Q -->b Abs x R by constructor.
+        by apply: (beta_step _ (Abs x Q) _ ).
+  Qed.
+
+  Lemma beta_stable_subst1 :
+    forall x M N N', N -->b N' -> subst x N M -->b* subst x N' M.
+  Proof.
+    move=> x M N N' HN. elim: M => [y|P IHP Q IHQ|y P IHP] /=.
+    - case: (x == y).
+      + by apply: beta1_beta.
+      + by constructor.
+    - have:
+        App (subst x N P) (subst x N Q)
+            -->b* App (subst x N' P) (subst x N Q)
+        by apply: beta_stable_appl.
+      move=> H1.
+      have:
+        App (subst x N' P) (subst x N Q)
+            -->b* App (subst x N' P) (subst x N' Q)
+        by apply: beta_stable_appr.
+      move=> H2.
+        by apply: (beta_transitive _ _ _ H1 H2).
+    - case: (x == y).
+      + by constructor.
+      + by apply: beta_stable_abs.
+  Qed.  
+
+  Lemma subst_comm : forall (x y : var) P Q N,
+      x != y -> y \notin freevars N ->
+      subst x N (subst y Q P) = subst y (subst x N Q) (subst x N P).
+  Proof.
+    move=> x y P Q N Hneq Hfvs.
+    elim: P => [z|P' IHP' Q' IHQ'|z P IHP'].
+    - rewrite /=. case E: (y == z).
+      + move/eqP: E => E. rewrite <- E.
+        move/negbTE: Hneq => Hneq.
+        by rewrite Hneq /= eq_refl.
+      + case E': (x == z).
+        * rewrite /= E'.
+            by apply subst_notin_fv.
+        * by rewrite /= E E'.
+    - by rewrite /= IHP' IHQ'.
+    - rewrite /=. case E1: (y==z); case E2: (x==z); rewrite /= E1 E2.
+      - by [].
+      - by [].
+      - 
+ 
+      
+  Lemma beta_stable_subst2 : 
+    forall x M M' N, M -->b M' -> subst x N M -->b* subst x N M'.
+  Proof.
+    move=> x M M' N. elim: M => [y| P IHP Q IHQ|y P IHP] /=.
+  Admitted.
+
+  Lemma redex_inv :
+    forall x M N Q, App (Abs x M) N -->b Q ->
+                    (exists M', App (Abs x M) N -->b App (Abs x M') N)
+                    \/ (exists N', App (Abs x M) N -->b App (Abs x M) N').
+  Proof.
+    move=> x M N Q. case: Q.
+    
+
+  Lemma diamond :
+    forall P Q Q', P -->b Q -> P -->b Q' -> exists R, Q -->b* R /\ Q' -->b* R.
+  Proof.
+    move=> P Q Q' H1 H2. move: Q' H2. elim H1.
+    + move=> x M N Q'.
+    
+
+(* Definition index := seq nat. *)
+
+(* Fixpoint is_valid_index (M : lterm) (idx : index) : bool := *)
+(*   match idx with *)
+(*   | [::] => true  *)
+(*   | i :: idx' => match M with *)
+(*                | Var x => false *)
+(*                | Abs x P => match i with *)
+(*                            | 0 => is_valid_index P idx' *)
+(*                            | _ => false *)
+(*                            end *)
+(*                | App P Q => match i with *)
+(*                            | 0 => is_valid_index P idx' *)
+(*                            | 1 => is_valid_index Q idx' *)
+(*                            | _ => false *)
+(*                            end *)
+(*                end *)
+(*   end. *)
+
+(* Fixpoint foo (n m : nat) := *)
+(*   match m with *)
+(*   | 0 => true *)
+(*   | S k => false && foo m k *)
+(*   end. *)
+
+(* Variable x : nat. *)
+(* Compute (foo x 0). *)
+
+(* Fixpoint bar n m := *)
+(*   match m with *)
+(*   | 0 => n *)
+(*   | S k => m *)
+(*   end. *)
+
+(* Compute bar n 0. *)
+
+
+
+(* Lemma bar : forall n, reflect True (foo n 0). *)
+(* Proof. *)
+(*   move=> n /=. simpl. *)
+
+
+
+(* Inductive valid_index : lterm -> index -> Prop := *)
+(* | valid_nil *)
+(*   : forall M, valid_index M nil *)
+(* | valid_abs *)
+(*   : forall x M idxM, valid_index M idxM -> valid_index (Abs x M) (0 :: idxM) *)
+(* | valid_appl *)
+(*   : forall M N idxM, valid_index M idxM -> valid_index (App M N) (0 :: idxM) *)
+(* | valid_appr *)
+(*   : forall M N idxN, valid_index N idxN -> valid_index (App M N) (1 :: idxN). *)
+
+(* Lemma valid_indexP : forall M idx, reflect (valid_index M idx) (is_valid_index M idx). *)
+(* Proof. *)
+(*   move=> M idx. *)
+(*   elim: idx. *)
+(*   - cbv. *)
+
+(*     case: M => [x|P Q|x P] /=; by constructor; constructor. *)
+(*   - move=> i idx'. case: M => [x|P Q|x P] /=. *)
+(*     + move=> IH. constructor. move=> Hv. elim E: Hv. *)
+      
+    
+(* Fixpoint get_opt (M : lterm) (idx : index) : option lterm := *)
+(*   match idx with *)
+(*   | nil => M *)
+(*   | i :: idx' => match M with *)
+(*                |  *)
+  
+(*   match M, idx with *)
+(*   | _, nil => Some M *)
+(*   | Abs x P, i :: idx' => match h with *)
+(*                      | 0 => get_opt P t *)
+(*                      | _ => None *)
+(*                      end *)
+(*   | App P Q, i :: idx => match h with *)
+(*                      | 0 => get_opt P t *)
+(*                      | 1 => get_opt Q t *)
+(*                      | _ => None *)
+(*                      end *)
+(*   | _, _ => None *)
+(*   end. *)
+
+(* Fixpoint replace_index (M : lterm) (idx : index) (N : lterm) : lterm := *)
+(*   match idx with *)
+(*   | nil => N *)
+(*   | i :: idx' *)
+
+(* Fixpoint i {M} (idxM : index M) (N : lterm) : option (index N) := *)
+(*   match idxM, N with *)
+(*   | index_root _, _ => Some (index_root _) *)
+(*   | _, _ => None *)
+(*   end. *)
+
+(* Inductive isomorphic_index : forall M N, index M -> index N -> Prop := *)
+(* | . *)
+
+
+(* Check (index_abs 1 _ (index_root (Abs 0 (Var 0)))). *)
+
+Section subst_op.
+  Variable subst : var -> lterm -> lterm.
+  Variable freevars : lterm -> varset.
+
+  
+
+                                             
+
+Fixpoint subst (x : var) (N M : lterm) :=
+  match M with
+  | Var y => if x == y
+            then N
+            else Var y
+  | App P Q => App (subst x N P) (subst x N Q)
+  | Abs y P => if x == y
+              then Abs y P
+              else Abs y (subst x N P)
+  end.
+
+Fixpoint ca_subst (x : var) (N M : lterm) : option lterm :=
+  match M with
+  | Var y => if x == y
+            then Some N
+            else Some (Var y)
+  | App P Q => match ca_subst x N P, ca_subst x N Q with
+              | Some P', Some Q' => Some (App P' Q')
+              | _, _ => None
+              end
+  | Abs y P => if x == y
+              then Some (Abs y P)
+              else if y \in (freevars N)
+                   then None
+                   else match ca_subst x N P with
+                        | Some P' => Some (Abs y P')
+                        | _ => None
+                        end
+  end.
+
+Fixpoint shift_f (f: nat -> nat) (d : nat) (M : lterm) : lterm :=
+  match M with
+  | Var x => if (PeanoNat.Nat.leb d x)
+            then Var (f x)
+            else Var x
+  | App P Q => App (shift_f f d P) (shift_f f d Q)
+  | Abs x P => Abs x (shift_f f (S d) P)
+  end.
+
+Definition shift_up := shift_f S 0.
+Definition shift_down := shift_f pred 0.
+  
+Fixpoint db_subst (x : var) (N M : lterm) : lterm :=
+  match M with
+  | Var y => if var_eq_dec x y
+            then N
+            else Var y
+  | App P Q => App (db_subst x N P) (db_subst x N Q)
+  | Abs y P => Abs y (db_subst (S x) (shift_up N) P)
+  end.
+
+Definition db_subst_redex (x : var) (M N : lterm) :=
+  shift_down (db_subst x (shift_up N) M).
+
+Inductive db_beta_reducible : lterm -> lterm -> Prop :=
+| dbbr_redex (x : var) (M N : lterm)
+  : db_beta_reducible (App (Abs x M) N)
+                      (db_subst_redex x N M)
+| dbbr_appl (M M' N : lterm)
+            (HM : db_beta_reducible M M')
+  : db_beta_reducible (App M N) (App M' N) 
+| dbbr_appr (M N N' : lterm)
+            (HN : db_beta_reducible N N')
+  : db_beta_reducible (App M N) (App M N')
+| dbbr_abs (x : var) (M M' : lterm)
+           (HM : db_beta_reducible M M')
+  : db_beta_reducible (Abs x M) (Abs x M').
+
+Inductive redex : lterm -> Prop :=
+| redex_intro (x : var) (M N : lterm)
+  : redex (App (Abs x M) N).
+
+Inductive immd_subterm : lterm -> lterm -> Prop :=
+| immd_subterm_appl (M N : lterm) : immd_subterm M (App M N)
+| immd_subterm_appr (M N : lterm) : immd_subterm N (App M N)
+| immd_subterm_abs (x : var) (M : lterm) : immd_subterm M (Abs x M).
+
+Inductive nf : lterm -> Prop :=
+| nf_var (x : var) : nf (Var x)
+| nf_app_var (x : var) (N : lterm) (HN : nf N)
+  : nf (App (Var x) N)
+| nf_app_app (P Q N : lterm) (HPQ : nf (App P Q))
+             (HN : nf N)
+  : nf (App (App P Q) N)
+| nf_abs (x : var) (M : lterm) (HM : nf M)
+  : nf (Abs x M).    
+
+Lemma nf_dec : forall M, {nf M} + {~ nf M}.
+Proof.
+  intros M. induction M.
+  - left. apply nf_var.
+  - destruct M1; destruct IHM2.
+    + left. apply nf_app_var. apply n.
+    + apply right. intros H. inversion H. contradiction.
+    + destruct IHM1. left. apply nf_app_app. apply n0. apply n.
+      right. intros H. inversion H. contradiction.
+    + right. intros H. inversion H. contradiction.
+    + right. intros H. inversion H.
+    + right. intros H. inversion H.
+  - destruct IHM. left. apply nf_abs. apply n.
+    right. intros H. inversion H. contradiction.
+Qed.
+
+Lemma not_nf : forall M,
+    ~ nf M
+    -> redex M
+      \/ (exists M', immd_subterm M' M /\ ~ nf M').
+Proof.
+  intros M Hnnf. destruct M as [].
+  - exfalso. apply Hnnf. apply nf_var.
+  - destruct M1 as [].
+    + assert (Hnnfm2 : ~ nf M2).
+      { intros Hnfm2. apply Hnnf.
+        apply nf_app_var. apply Hnfm2. }
+      right. exists M2. split. apply immd_subterm_appr.
+      apply Hnnfm2.
+    + destruct (nf_dec M2).
+      * assert (Hnnfapp : ~ nf (App M1_1 M1_2)).
+        { intros Hnfapp. apply Hnnf. apply nf_app_app.
+          auto. auto. }
+        right. exists (App M1_1 M1_2). split.
+        apply immd_subterm_appl. auto.
+      * right. exists M2. split. apply immd_subterm_appr.
+        auto.
+    + left. apply redex_intro.
+  - right. assert (HnnfM : ~ nf M).
+    { intros HnfM. apply Hnnf. apply nf_abs. auto. }
+    exists M. split. apply immd_subterm_abs. auto.
+Qed.
+    
+      
+Lemma nf_not_exists : forall M, nf M -> ~ exists M', db_beta_reducible M M'.
+Proof.
+  intros M Hnf. induction Hnf.
+  - intros [M' HM']. inversion HM'.
+  - intros [M' HM']. inversion HM'.
+    inversion HM. apply IHHnf. exists N'. apply HN.
+  - intros [M' HM']. inversion HM'.
+    apply IHHnf1. exists M'0. apply HM.
+    apply IHHnf2. exists N'. apply HN.
+  - intros [M' HM']. inversion HM'.
+    apply IHHnf. exists M'0. apply HM.
+Qed.
+
+Lemma redex_reducible : forall M,
+    redex M -> exists M', db_beta_reducible M M'.
+Proof.
+  intros _ [x M N]. exists (db_subst_redex x N M). 
+  apply dbbr_redex.
+Qed.
+
+Lemma not_nf_exists : forall M, ~ nf M -> exists M', db_beta_reducible M M'.
+Proof.
+  intros M Hnnf. induction M.
+  - exfalso. apply Hnnf. apply nf_var.
+  - apply not_nf in Hnnf. destruct Hnnf as [Hredex|Hnredex].
+    + apply redex_reducible in Hredex.
+      apply Hredex.
+    + destruct Hnredex as [M' [Hsub HnnfM']].
+      inversion Hsub.
+      * rewrite H1 in HnnfM'.
+        apply IHM1 in HnnfM'.
+        destruct HnnfM' as [M1' HM1'].
+        exists (App M1' M2). apply dbbr_appl. auto.
+      * rewrite H2 in HnnfM'.
+        apply IHM2 in HnnfM'.
+        destruct HnnfM' as [M2' HM2'].
+        exists (App M1 M2'). apply dbbr_appr. auto.
+  - apply not_nf in Hnnf. destruct Hnnf as [Hredex|Hnredex].
+    + inversion Hredex.    
+    + destruct Hnredex as [M' [Hsub HM']].
+      inversion Hsub. rewrite H2 in HM'. apply IHM in HM'.
+      destruct HM' as [M'' HM''].
+      exists (Abs x M''). apply dbbr_abs. apply HM''.
+Qed.
+
+Inductive bigstep : lterm -> lterm -> Prop :=
+| bigstep_nf : forall M,
+    nf M
+    -> bigstep M M
+| bigstep_abs : forall x M M',
+    bigstep M M'
+    -> bigstep (Abs x M) (Abs x M')
+| bigstep_abs_app : forall x M M' N P,
+    bigstep M (Abs x M') -> bigstep (db_subst_redex x N M') P
+    -> bigstep (App M N) P
+| bigstep_var_app : forall x M N N',
+    bigstep M (Var x) -> bigstep N N'
+    -> bigstep (App M N) (App (Var x) N')
+| bigstep_app_app : forall M P Q N N',
+    bigstep M (App P Q) -> bigstep N N'
+    -> bigstep (App M N) (App (App P Q) N').
+
+Notation "M ⇓ N" := (bigstep M N) (at level 70).
+Notation "M ->b N" := (db_beta_reducible M N) (at level 70).
+Notation "M ->b* N" := (clos_refl_trans_1n _ db_beta_reducible M N) (at level 70).
+
+Lemma bigstep_to_nf : forall M N, M ⇓ N -> nf                                                               N. 
+Proof.
+  intros M N Hstep. induction Hstep.
+  - auto.
+  - apply nf_abs. auto.
+  - auto.
+  - apply nf_app_var. auto.
+  - apply nf_app_app. auto. auto.
+Qed.
+
+(* Lemma multistep_bigstep : forall M N, (M ->b* N) -> nf N -> M ⇓ N. *)
+(* Proof. *)
+(*   intros M N Hmultistep Hnf. induction Hmultistep. *)
+(*   - apply bigstep_nf. auto. *)
+(*   - apply IHHmultistep in Hnf. inversion Hnf. *)
+
+(* Lemma bigstep_neq : forall M N, M ⇓ N -> M <> N -> ~ nf M. *)
+
+Lemma bigstep_deterministic : forall M P Q, M ⇓ P -> M ⇓ Q -> P = Q.
+Proof.
+  intros M P Q HMP HMQ. induction HMP.
+  - inversion HMQ. reflexivity.
+  
+  - intros P Q HMP HMQ. inversion HMP. inversion HMQ. reflexivity.
+  - intros P Q HMP HMQ. inversion HMP.
+    + inversion H.
+      
+Inductive db_beta_reducibleT : lterm -> lterm -> Type :=
+| dbbr_redexT (x : var) (M N : lterm)
+  : db_beta_reducibleT (App (Abs x M) N)
+                      (db_subst_redex x N M)
+| dbbr_applT (M M' N : lterm)
+            (HM : db_beta_reducibleT M M')
+  : db_beta_reducibleT (App M N) (App M' N)
+| dbbr_apprT (M N N' : lterm)
+            (HN : db_beta_reducibleT N N')
+  : db_beta_reducibleT (App M N) (App M N')
+| dbbr_absT (x : var) (M M' : lterm)
+           (HM : db_beta_reducibleT M M')
+  : db_beta_reducibleT (Abs x M) (Abs x M').
+
+Definition derivation := { M : lterm & { N : lterm & db_beta_reducible M N} }.
+
+Inductive isd : derivation -> derivation -> Prop :=
+| isd_appl : forall M M' N (d : db_beta_reducibleT M M'),
+    isd (existT 
+
+Fixpoint depth {M N} (d : db_beta_reducibleT M N) : nat :=
+  match d with
+  | dbbr_redexT _ _ _ => 0
+  | dbbr_applT _ _ _ d' => S (depth d')
+  | dbbr_apprT _ _ _ d' => S (depth d')
+  | dbbr_absT _ _ _ d' => S (depth d')
+  end.
+
+Definition derivation_prop := forall M N, db_beta_reducibleT M N -> Prop.
+
+Definition thing (P : derivation_prop) (n : nat) :=
+  forall M N (d : db_beta_reducibleT M N), depth d = n -> P M N d.
+
+Lemma depth_induciton : forall (P : derivation_prop),
+    (forall M N (dx : db_beta_reducibleT M N),
+        (forall M' N' (dy : db_beta_reducibleT M' N'),
+            depth dy < depth dx -> P _ _ dy)
+           -> P _ _ dx)
+    -> forall M N (dx : db_beta_reducibleT M N), P _ _ dx.
+Proof.
+  intros P Hind.
+  
+  assert (H : forall n, thing P n).
+  { apply (well_founded_ind Nat.lt_wf_0).
+    intros x Hx. unfold thing.
+    intros M N d Hd. apply Hind.
+    intros M' N' dy Hdy.
+    assert (H2 : thing P (depth dy)).
+    { apply Hx. rewrite Hd in Hdy. apply Hdy. }
+    unfold thing in H2. apply H2.
+    reflexivity. }
+  intros M N dx. unfold thing in H. apply H
+  with (n:= depth dx). reflexivity.
+Qed.
+
+Definition lex_lt (p1 p2 : nat * nat) : Prop :=
+  let (px1, py1) := p1 in
+  let (px2, py2) := p2 in
+  px1 < px2 \/ (px1 = px2 /\ py1 < py2).
+
+Lemma wf_lex_lt : well_founded lex_lt.
+Proof.
+  assert (H1 : forall y, Acc lex_lt (0, y)).
+  { apply (well_founded_ind Nat.lt_wf_0).
+    intros x IH. destruct x.
+    - apply Acc_intro. intros [x' y'] Hp.
+      simpl in Hp. destruct Hp. inversion H.
+      destruct H as [_ H]. inversion H.
+    - apply Acc_intro. intros [x' y'] Hp.
+      simpl in Hp. destruct Hp. inversion H.
+      destruct H as [Hx' Hy']. rewrite Hx'.
+      apply IH. apply Hy'. }
+  assert (H2 : forall y, (forall x, Acc lex_lt (x, y))).
+  { apply (well_founded_ind Nat.lt_wf_0).
+    intros x. intros IH.
+
+
+    destruct x. intros _. apply H1.
+    intros IH. apply Acc_intro.
+    intros p. destruct p as [x' y'].
+    
+    simpl. intros Hp. destruct Hp.
+    - apply IH in H.
+    
+  intros p. destruct p as [x y].
+
+  
+  apply (well_founded_ind Nat.lt_wf_0).
+  - intros x' IH. apply (well_founded_ind Nat.lt_wf_0). Admitted.
+  
+  
+    (* induction y. *)
+    (* + apply Acc_intro. intros [x' y'] Hp'. *)
+    (*   simpl in Hp'. destruct Hp' as []. *)
+    (*   inversion H. destruct H as [_ H]. inversion H. *)
+    (* + apply Acc_intro. intros [x' y']. simpl. intros H. *)
+    (*   inversion IHy. destruct H. inversion H. *)
+    (*   destruct H as [Hx' Hy']. rewrite Hx'. *)
+    (*   destruct (Nat.compare y y') as [| |] eqn:E. *)
+    (*   * apply Nat.compare_eq in E. rewrite <- E. *)
+    (*     apply IHy. *)
+    (*   * apply Nat.compare_lt_iff in E. *)
+    (*     apply H0. simpl. right. Admitted. *)
+
+Lemma wf_diag : well_founded (fun (p1 p2 : nat * nat) => let (x1, y1) := p1 in
+                                                  let (x2, y2) := p2 in
+                                                  x1 < x2 /\ y1 < y2).
+
+intros p. 
+
+                           
+      
+  
+Definition
+  immd_subderivation (sd1 sd2 : { d | exists P Q, d = db_beta_reducibleT P Q }) : Prop :=
+  let (d1, Hd1) := sd1 in
+  let (d2, Hd2) := sd2 in
+  (exists M M' N, d2 = dbbr_applT M M' N d1).
+
+Inductive immd_subderivation
+          (d1 d2 : { d | exists P Q, d = db_beta_reducible P Q }) : Prop :=
+| immd_sd_appl (H : exists M M' N, proj1_sig d2 = dbbr_applT M M' N (proj2_sig d1))
+  : immd_subderivation d1 d2.
+
+Lemma immd_subderivation_wf : forall p q r s,
+    well_founded (immd_subderivation p q r s).
+  
+  
+Lemma diamond : forall M P Q,
+    db_beta_reducible M P
+    -> db_beta_reducible M Q
+    -> P = Q \/ exists R, db_beta_reducible P R /\ db_beta_reducible Q R.
+Proof.
+  intros M P Q HMP HMQ. 
