Weird.v
@@ -1,0 +1,26 @@
+Variable f : bool -> bool.
+Variable x : nat.
+
+Fixpoint foo (n m : nat) :=
+  match m with
+  | 0 => true
+  | S k => f (foo n k)
+  end.
+
+Fixpoint bar (n m : nat) :=
+  match m with
+  | 0 => true
+  | S k => (fun _ => true) (bar n k)
+  end.
+
+Fixpoint quux (g : bool -> bool) (n m : nat) :=
+  match m with
+  | 0 => true
+  | S k => g (quux g n k)
+  end.
+
+Compute foo x 0.
+Compute bar x 0.
+Compute quux f x 0.
+Compute quux (fun _ => true) x 0.
+Eval cbv delta iota in quux (fun _ => true) x 0. 
